Update plain unfolding to allow for later credits. The HasNoLC is still needed in adequacy as the progress and preservation proofs are not yet seperate

trillium/program_logic/plain_unfolding.v
@@ -10,6 +10,14 @@ Import le_upd_if.
 
 Section plain_unfolding.
 
+  Global Instance is_except_0_laterN {Σ} n (P : iProp Σ) :
+    IsExcept0 P →
+    IsExcept0 (▷^n P).
+  Proof.
+    destruct n; [done|].
+    simpl; tc_solve.
+  Qed.
+
   Local Lemma lc_incr_supply `{!lcGS Σ} n m :
     later_credits.lc_supply n ⊢ |==> later_credits.lc_supply (n + m) ∗ £ m.
   Proof.
@@ -18,6 +26,9 @@ Section plain_unfolding.
     iApply (own_update with "[$]").
     eapply auth_update. eapply nat_local_update; lia.
   Qed.
+
+
+  (* In case of no later credit update. *)
 
   Definition lc_generator_aux `{lcGS Σ} (rec : unit → iProp Σ) (_ : unit) : iProp Σ :=
     ∀ (P : iProp Σ) n, (£ n -∗ rec () -∗ P) ==∗ P.
@@ -50,19 +61,113 @@ Section plain_unfolding.
     iApply ("HP" with "[$] [$]").
   Qed.
 
+  (* In case of later credit update *)
+
+  Definition le_upd_to_bupd_aux `{!lcGS Σ}
+      (rec : nat → iProp Σ) (n : nat) : iProp Σ :=
+    ∀ (P : iProp Σ) `(!Plain P) `(!IsExcept0 P) m, ((£ m -∗ |==£> ∀ k, rec k -∗ ▷^k P) -∗ ▷^(n+m) P).
+  
+  Definition le_upd_to_bupd `{!lcGS Σ} n :=
+    bi_greatest_fixpoint le_upd_to_bupd_aux n.
+  
+  Instance le_upd_to_bupd_aux_bi_mono `{!lcGS Σ} :
+    BiMonoPred (le_upd_to_bupd_aux).
+  Proof.
+    split.
+    - iIntros (Φ Ψ HΦne HΨne) "#H". iIntros (n) "Hn". iIntros (P ? ? m) "HP /=".
+      iApply "Hn"; try (iPureIntro; tc_solve). iIntros "?".
+      iMod ("HP" with "[$]") as "HP". iIntros "!> %k HΦ"; iApply "HP"; by iApply "H".
+    - iIntros (Φ HΦne). by intros ??? ->.
+  Qed.
+
+  Lemma le_upd_to_bupd_unfold `{!lcGS Σ} n :
+    le_upd_to_bupd n ≡ le_upd_to_bupd_aux le_upd_to_bupd n.
+  Proof. by rewrite /le_upd_to_bupd greatest_fixpoint_unfold. Qed.
+
+
+  Definition le_upd_to_bupd_use `{!lcGS Σ} n m P `{!IsExcept0 P} `{!Plain P} :
+    le_upd_to_bupd n -∗ (£ m -∗ |==£> ∀ k, le_upd_to_bupd k -∗ ▷^k P) -∗ ▷^(n + m) P.
+  Proof.
+    iIntros "Hn HP". rewrite le_upd_to_bupd_unfold.
+    iApply ("Hn" with "[] [] HP"); try (iPureIntro; tc_solve).
+  Qed.
+  
+  Lemma le_upd_to_bupd_soundness_lc `{!lcGpreS Σ} P `{!IsExcept0 P} `{!Plain P} :
+    (∀ `{Hlc: !lcGS Σ}, le_upd_to_bupd 0 -∗ P) → ⊢ P.
+  Proof.
+    iIntros (Hfupd).
+    iMod (later_credits.le_upd.lc_alloc 0) as (Hc) "[H _]".
+    iApply (Hfupd _). generalize 0 => n.
+    iApply (greatest_fixpoint_coiter _ later_credits.lc_supply with "[] [$H]").
+    iIntros "!> % Hsup %Q % % %m HQ". iApply bupd_elim.
+    iMod (lc_incr_supply _ m with "Hsup") as "[Hsup Hlc]".
+    iSpecialize ("HQ" with "Hlc"). clear n. generalize (y + m) => n. clear y m.
+    iLöb as "IH" forall (n).
+    iEval (rewrite later_credits.le_upd.le_upd_unfold) in "HQ".
+    iMod ("HQ" with "[$]") as "[[Hsup Hrest]|(%m&%Hmle&Hsup&Hnext)]".
+    - iModIntro. iApply is_except_0.
+      iDestruct ("Hrest" with "[$]") as "$".
+    - destruct n as [|n]; [lia|simpl].
+      do 2 iModIntro.
+      iApply (bi.laterN_le m); [lia|].
+      iApply bupd_elim.
+      iApply ("IH" with "[$] [$]").
+  Qed.
+
+  (* Either *)
+
+  Local Definition le_upd_if_to_bupd_def `{!lcGS Σ} (hlc : has_lc) n :=
+    match hlc with
+    | HasLc => le_upd_to_bupd n
+    | HasNoLc => lc_generator ()
+    end.
+  Local Definition le_upd_if_to_bupd_aux : seal (@le_upd_if_to_bupd_def). Proof. by eexists. Qed.
+  Definition le_upd_if_to_bupd := le_upd_if_to_bupd_aux.(unseal).
+  Local Definition le_upd_if_to_bupd_unseal :
+    @le_upd_if_to_bupd = @le_upd_if_to_bupd_def := le_upd_if_to_bupd_aux.(seal_eq).
+  Global Arguments le_upd_if_to_bupd {_ _} hlc n.
+
+  Definition has_lc_to_bool (hlc : has_lc) :=
+    match hlc with
+    | HasLc => true
+    | HasNoLc => false
+    end.
+
+  Definition le_upd_if_to_bupd_use `{!lcGS Σ} hlc n m P `{!IsExcept0 P} `{!Plain P} :
+    le_upd_if_to_bupd hlc n -∗ (£ m -∗ le_upd_if (has_lc_to_bool hlc) (∀ k, le_upd_if_to_bupd hlc k -∗ ▷^k P)) -∗ ▷^(m + n) P.
+  Proof.
+    rewrite (comm _ m n). rewrite le_upd_if_to_bupd_unseal.
+    destruct hlc; [by apply le_upd_to_bupd_use|].
+    simpl. iIntros "Hgen Hupd".
+    iApply bupd_elim. iEval (rewrite lc_generator_unfold) in "Hgen".
+    iApply "Hgen". iIntros "H£ Hgen".
+    iMod ("Hupd" with "[$]") as "Hupd".
+    by iApply "Hupd".
+  Qed.
+
+  Lemma le_upd_if_to_bupd_soundness `{!lcGpreS Σ} hlc P `{!IsExcept0 P} `{!Plain P} :
+    (∀ `{Hlc: !lcGS Σ}, le_upd_if_to_bupd hlc 0 -∗ P) → ⊢ P.
+  Proof.
+    rewrite le_upd_if_to_bupd_unseal.
+    destruct hlc; [by apply le_upd_to_bupd_soundness_lc|].
+    intros. iApply bupd_elim. by iApply lc_generator_soundness_no_lc.
+  Qed.
+
+
   Definition fupd_to_bupd_aux `{invGS_gen hlc Σ}
            (rec : coPset → iProp Σ) (E1 : coPset) : iProp Σ :=
-    ∀ (P : iProp Σ) E2, ((|={E1,E2}=> rec E2 -∗ P) ==∗ ◇ P).
+    ∀ (P : iProp Σ) `(!Plain P) `(!IsExcept0 P) n E2, le_upd_if_to_bupd hlc n -∗ ((|={E1,E2}=> ∀ k, le_upd_if_to_bupd hlc k -∗ rec E2 -∗ ▷^k P) -∗ ▷^n P).
 
-  Definition fupd_to_bupd `{invGS_gen hlc Σ} :=
-    bi_greatest_fixpoint fupd_to_bupd_aux.
+  Definition fupd_to_bupd `{invGS_gen hlc Σ} E1 :=
+    bi_greatest_fixpoint fupd_to_bupd_aux E1.
 
   Instance fupd_to_bupd_aux_bi_mono `{invGS_gen hlc Σ} :
     BiMonoPred (fupd_to_bupd_aux).
   Proof.
     split.
-    - iIntros (Φ Ψ HΦne HΨne) "#H". iIntros (E1) "HE". iIntros (P E2) "HP".
-      iApply "HE"; iMod "HP"; iModIntro. by iIntros; iApply "HP"; iApply "H".
+    - iIntros (Φ Ψ HΦne HΨne) "#H". iIntros (E1) "HE". iIntros (P ? ? n E2) "Hle HP /=".
+      iApply ("HE" with "[] [] Hle"); try (iPureIntro; tc_solve); iMod "HP"; iModIntro.
+      iIntros; iApply ("HP" with "[$]"); by iApply "H".
     - iIntros (Φ HΦne). by intros ??? ->%leibniz_equiv.
   Qed.
 
@@ -70,75 +175,78 @@ Section plain_unfolding.
     fupd_to_bupd E ≡ fupd_to_bupd_aux fupd_to_bupd E.
   Proof. by rewrite /fupd_to_bupd greatest_fixpoint_unfold. Qed.
 
-  Lemma fupd_to_bupd_except0 `{invGS_gen hlc Σ} E E' P `{!IsExcept0 P} :
+  (* Lemma fupd_to_bupd_except0 `{invGS_gen hlc Σ} E E' P `{!IsExcept0 P} :
     fupd_to_bupd E -∗ (|={E, E'}=> fupd_to_bupd E' -∗ P) ==∗ P.
   Proof.
     iIntros "HE HP". rewrite fupd_to_bupd_unfold.
     iApply (is_except_0 P). iApply ("HE" with "[$]").
+  Qed. *)
+
+  Lemma fupd_to_bupd_except0_plain `{invGS_gen hlc Σ} n E E' P `{!IsExcept0 P} `{!Plain P} :
+    fupd_to_bupd E -∗ le_upd_if_to_bupd hlc n -∗ (|={E, E'}=> ∀ k, le_upd_if_to_bupd hlc k -∗ fupd_to_bupd E' -∗ ▷^k P) -∗ ▷^n P.
+  Proof.
+    iIntros "HE Hle HP". rewrite fupd_to_bupd_unfold.
+    iDestruct ("HE" with "[] [] Hle HP") as "H"; by try (iPureIntro; tc_solve).
   Qed.
 
-  Lemma fupd_to_bupd_except0_plain `{invGS_gen hlc Σ} E E' P `{!IsExcept0 P} `{!Plain P} :
-    fupd_to_bupd E -∗ (|={E, E'}=> fupd_to_bupd E' -∗ P) -∗ P.
+  Lemma fupd_to_bupd_soundness `{!invGpreS Σ} hlc P `{!IsExcept0 P} `{!Plain P} :
+    (∀ `{Hinv: !invGS_gen hlc Σ}, le_upd_if_to_bupd hlc 0 -∗
+      fupd_to_bupd ⊤ -∗ P) → ⊢ P.
   Proof.
-    iIntros "HE HP". iApply bupd_elim. iApply (fupd_to_bupd_except0 with "[$] [$]").
-  Qed.
-
-  Lemma fupd_to_bupd_soundness_no_lc `{!invGpreS Σ} (Q : iProp Σ) :
-    (∀ `{Hinv: !invGS_gen HasNoLc Σ}, lc_generator () -∗
-      fupd_to_bupd ⊤ -∗ Q) → ⊢ |==> Q.
-  Proof.
-    iIntros (Hfupd). iApply bupd_trans.
-    iApply (@lc_generator_soundness_no_lc _ invGpreS_lc).
+    iIntros (Hfupd). iApply bupd_elim.
+    iApply (@le_upd_if_to_bupd_soundness _ invGpreS_lc).
     iIntros (Hc) "Hgen".
     iMod ( @wsat_alloc _ (invGpreS0.(invGpreS_wsat))) as (Hw) "[Hw HE]".
-    set (Hi := InvG HasNoLc _ Hw Hc).
+    set (Hi := InvG hlc _ Hw Hc).
     iApply ( @Hfupd Hi with "Hgen").
     assert (NonExpansive (λ E, wsat ∗ ownE E)%I).
     { by intros ??? ->%leibniz_equiv. }
     iApply (greatest_fixpoint_coiter _ (λ E, wsat ∗ ownE E)%I with "[] [$Hw $HE]").
-    iIntros "!>" (E1) "?".
-    iIntros (P E2) "HP".
+    iIntros "!>" (E1) "?". clear.
+    iIntros (P ? ? ? E2) "Hle HP".
     rewrite fancy_updates.uPred_fupd_unseal /fancy_updates.uPred_fupd_def /=.
-    iMod ("HP" with "[$]") as ">(Hw & HE & HP)".
-    do 2 iModIntro; iApply "HP"; iFrame.
+    iApply (le_upd_if_to_bupd_use _ _ 0 with "[$]"). iIntros "H".
+    iMod ("HP" with "[$]") as "Hrest".
+    iIntros "!> %k Hle". iMod "Hrest" as "(?&?&Hclose)".
+    iApply ("Hclose" with "[$Hle] [$]").
   Qed.
 
   (* TODO: Make this opaque *)
   Definition step_count `{!tr_generation} (ns : nat) : nat :=
-    S $ f $ physical_step.tr_per_step 0 ns.
+    let trs := physical_step.tr_per_step 0 ns in
+    (f $ S $ trs) + (S $ f $ trs).
 
-  Definition physical_step_to_laters_aux `{!tr_generation} `{invGS_gen HasNoLc Σ} `{trGS Σ} (rec : nat → iProp Σ) (ns : nat) : iProp Σ :=
-    ∀ (P : iProp Σ) (E : coPset), (fupd_to_bupd E -∗ (|={E}⧗=> fupd_to_bupd E -∗ rec (S ns) -∗ ◇■ P) -∗ ▷^(step_count ns) ◇■ P).
+  Definition physical_step_to_laters_aux `{!tr_generation} `{invGS_gen hlc Σ} `{trGS Σ} (rec : nat → iProp Σ) (ns : nat) : iProp Σ :=
+    ∀ (P : iProp Σ) `(!Plain P) `(!IsExcept0 P) n (E : coPset), (fupd_to_bupd E -∗ le_upd_if_to_bupd hlc n -∗ (|={E}⧗=> ∀ k, fupd_to_bupd E -∗ le_upd_if_to_bupd hlc k -∗ rec (S ns) -∗ ▷^k P) -∗ ▷^(step_count ns + n) P).
   
-  Definition physical_step_to_laters `{!tr_generation} `{invGS_gen HasNoLc Σ} `{trGS Σ} :=
+  Definition physical_step_to_laters `{!tr_generation} `{invGS_gen hlc Σ} `{trGS Σ} :=
     bi_greatest_fixpoint physical_step_to_laters_aux.
   
-  Instance physical_step_to_laters_aux_bi_mono `{!tr_generation} `{invGS_gen HasNoLc Σ} `{trGS Σ} :
+  Instance physical_step_to_laters_aux_bi_mono `{!tr_generation} `{invGS_gen hlc Σ} `{trGS Σ} :
     BiMonoPred (physical_step_to_laters_aux).
   Proof.
     split.
-    - iIntros (Φ Ψ HΦne HΨne) "#H". iIntros (n) "Hn". iIntros (P E) "HE HP".
-      iApply ("Hn" with "[$]"). iApply (physical_step_wand with "[$]"). iIntros "HP ? ?".
-      iApply ("HP" with "[$]"). by iApply "H".
+    - iIntros (Φ Ψ HΦne HΨne) "#H". iIntros (ns) "Hns". iIntros (P ? ? n E) "HE Hle HP".
+      iApply ("Hns" with "[] [] [$] [$]"); try (iPureIntro; tc_solve).
+      iApply (physical_step_wand with "[$]"). iIntros "HP %k ? ? ?".
+      iApply ("HP" with "[$] [$]"). by iApply "H".
     - iIntros (Φ HΦne). by intros ??? ->%leibniz_equiv.
   Qed.
 
-  Lemma physical_step_to_laters_unfold `{!tr_generation} `{invGS_gen HasNoLc Σ} `{trGS Σ} ns :
+  Lemma physical_step_to_laters_unfold `{!tr_generation} `{invGS_gen hlc Σ} `{trGS Σ} ns :
     physical_step_to_laters ns ≡ physical_step_to_laters_aux physical_step_to_laters ns.
   Proof. by rewrite /physical_step_to_laters greatest_fixpoint_unfold. Qed.
 
-  Lemma physical_step_to_laters_except0_plain `{!tr_generation} `{invGS_gen HasNoLc Σ} `{trGS Σ} ns E P `{!IsExcept0 P} `{!Plain P} :
-    physical_step_to_laters ns -∗ fupd_to_bupd E -∗ (|={E}⧗=> fupd_to_bupd E -∗ physical_step_to_laters (S ns) -∗ P) -∗ ▷^(step_count ns) P.
+  Lemma physical_step_to_laters_except0_plain `{!tr_generation} `{invGS_gen hlc Σ} `{trGS Σ} ns n E P `{!IsExcept0 P} `{!Plain P} :
+    physical_step_to_laters ns -∗ fupd_to_bupd E -∗ le_upd_if_to_bupd hlc n -∗ (|={E}⧗=>  ∀ k, fupd_to_bupd E -∗ le_upd_if_to_bupd hlc k -∗ physical_step_to_laters (S ns) -∗ ▷^k P) -∗ ▷^(step_count ns + n) P.
   Proof.
-    iIntros "Hsteps Hfupd HP".
-    iApply (bi.laterN_wand _ (◇■ P)%I).
-    { iNext. iIntros. iApply is_except_0. iApply plainly_elim. by iApply except_0_plainly_1. }
-    rewrite physical_step_to_laters_unfold. iApply ("Hsteps" with "[$]").
-    iApply (physical_step_wand with "[$]"). iIntros "HP ? ?".
-    iApply bi.except_0_intro. iApply plain. by iApply ("HP" with "[$] [$]").
+    iIntros "Hsteps Hfupd Hle HP".
+    rewrite physical_step_to_laters_unfold.
+    iApply ("Hsteps" with "[] [] [$] [$]"); try (iPureIntro; tc_solve).
+    iApply (physical_step_wand with "[$]"). iIntros "$".
   Qed.
 
-  Lemma foo `{invGS_gen HasNoLc Σ} {E} E' n P :
+  (* Lemma foo `{invGS_gen HasNoLc Σ} {E} E' n P :
     fupd_to_bupd E -∗ (|={E, E'}=> fupd_to_bupd E' -∗ |==> ▷^n ◇ P) -∗ |==> ▷^n ◇ P.
   Proof.
     iIntros "HE HP".
@@ -150,67 +258,52 @@ Section plain_unfolding.
       iApply (fupd_to_bupd_unfold with "HE"). iMod "HP". iIntros "!> HE".
       iApply bi.except_0_intro.
       by iApply "HP".
-  Qed.
+  Qed. *)
 
-  Lemma bar `{invGS_gen Σ} n Q `{!Plain Q} `{!IsExcept0 Q} :
-    fupd_to_bupd ∅  -∗ (|={∅}▷=>^n fupd_to_bupd ∅ -∗ Q) -∗ (▷^n Q).
+  Lemma bar `{invGS_gen hlc Σ} n m Q `{!Plain Q} `{!IsExcept0 Q} :
+    fupd_to_bupd ∅ -∗ le_upd_if_to_bupd hlc m -∗ (|={∅}▷=>^n fupd_to_bupd ∅ -∗ ∀ k, le_upd_if_to_bupd hlc k -∗ ▷^k Q) -∗ (▷^(n + m) Q).
   Proof.
-    iIntros "HFtB HP".
-    iInduction n as [|n] "IHn".
-    { simpl. 
-      iApply is_except_0.
-      iApply bupd_elim.
-      rewrite {1}fupd_to_bupd_unfold.
-      iApply "HFtB". iApply "HP". }
-    simpl.
-    iApply bi.except_0_later.
-    iApply bupd_elim.
-    rewrite {3}fupd_to_bupd_unfold.
-    iApply "HFtB".
-    iMod "HP".
-    iIntros "!> HFtB !>".
-    iApply is_except_0.
-    { by destruct n; apply _. }
-    iApply bupd_elim.
-    rewrite {4}fupd_to_bupd_unfold.
-    iApply "HFtB".
-    iMod "HP".
-    iIntros "!> HFtB".
-    iApply ("IHn" with "HFtB HP").
+    rewrite (comm _ n m).
+    iIntros "HFtB Hle HP".
+    iInduction n as [|n] "IHn" forall (m).
+    { rewrite Nat.add_0_r. iApply ("HP" with "[$] [$]"). }
+    iEval (rewrite bi.laterN_add).
+    iApply (fupd_to_bupd_except0_plain with "[$] [$]"). iMod "HP". clear m.
+    iIntros "!> %m Hle HFtB". rewrite -bi.laterN_later bi.later_laterN.
+    iNext.
+    iApply (fupd_to_bupd_except0_plain with "[$] [$]"). iMod "HP". clear m.
+    iIntros "!> %m Hle HFtB". rewrite -bi.laterN_add.
+    iApply ("IHn" with "[$] [$] [$]").
   Qed.
-
-  Lemma except_0_laterN `{invGS_gen HasNoLc Σ} n (P : iProp Σ) :
-    n ≥ 1 →
-    ◇ ▷^n P ⊢ ▷^n P.
-  Proof.
-    intros ?. destruct n; [lia|].
-    simpl. apply bi.except_0_later.
-  Qed.  
 
   
-  Lemma physical_step_to_laters_soundness_no_lc  `{!tr_generation} `{!invGpreS Σ} `{trGpreS Σ} (Q : iProp Σ) :
-    (∀ `{invGS_gen HasNoLc Σ} `{trGS Σ}, fupd_to_bupd ⊤ -∗ physical_step_to_laters 0 -∗ Q) →
-    ⊢ |==> Q.
+  Lemma physical_step_to_laters_soundness  `{!tr_generation} `{!invGpreS Σ} `{trGpreS Σ} hlc Q `{!Plain Q} `{!IsExcept0 Q} :
+    (∀ `{invGS_gen hlc Σ} `{trGS Σ}, fupd_to_bupd ⊤ -∗ le_upd_if_to_bupd hlc 0 -∗ physical_step_to_laters 0 -∗ Q) →
+    ⊢ Q.
   Proof.
-    iIntros (Hfupd). iApply bupd_trans. iApply fupd_to_bupd_soundness_no_lc.
+    iIntros (Hfupd).
+    iApply (fupd_to_bupd_soundness hlc).
     iIntros (Hinv) "Hlc Hfupd".
     iMod (tr_supply_alloc 0) as "(%Htr & Hsup & H⧗)"; simpl.
-    iApply ( @Hfupd _ _ with "[$]").
-    assert (NonExpansive (λ n, lc_generator () ∗ tr_supply (physical_step.tr_per_step 0 n))%I).
+    iApply ( @Hfupd _ _ with "[$] [$]").
+    assert (NonExpansive (λ n, tr_supply (physical_step.tr_per_step 0 n))%I).
     { intros ????; repeat f_equiv; eauto. }
     iApply (greatest_fixpoint_coiter _
-      (λ n, lc_generator () ∗ tr_supply (physical_step.tr_per_step 0 n))%I with "[] [Hlc Hsup]"); [|iFrame].
-    iIntros "!>" (n) "[Hlc Htr]". rewrite /physical_step_to_laters_aux.
-    iIntros (P E) "HE HP". rewrite physical_step.physical_step_unseal /physical_step_def.
-    iApply bupd_elim. iApply (foo ∅ with "HE"). iMod "HP". iIntros "!> HE".
+      (λ n, tr_supply (physical_step.tr_per_step 0 n))%I with "[] [Hsup]"); [|iFrame].
+    iIntros "!>" (n) "Htr". rewrite /physical_step_to_laters_aux.
+    iIntros (P ? ? m E) "HE Hlc HP". rewrite physical_step.physical_step_unseal /physical_step_def.
+    unfold step_count. rewrite -assoc (comm _ _ m) assoc bi.laterN_add.
+    iApply (le_upd_if_to_bupd_use with "[$]"). iIntros "Hlc !> %k Hlc'".
+    iApply (fupd_to_bupd_except0_plain with "[$] [$]").
+    iMod "HP". clear k. iIntros "!> %k Hle HE".
     iMod tr_zero as "H⧗". iMod (tr_persistent_zero) as "H⧖".
-    iApply bupd_trans. iApply (lc_generator_unfold with "Hlc"). iIntros "H£ Hlc".
     iSpecialize ("HP" $! _ _ _ with "[$] [$] [$] [$]").
-    (* rewrite Nat.sub_0_r. fold (step_count n). iModIntro. *)
-    iApply (bar with "[$]"). iApply (step_fupdN_wand with "[$]").
-    iIntros "!> (Hsup&_&_&_&HP) HE".
-    iApply bupd_elim. iApply (foo E 0 with "HE"). iMod "HP". iIntros "!> HE !>".
-    iApply ("HP" with "[$] [$]").
+    rewrite -bi.later_laterN -bi.laterN_add (comm _ k).
+    iApply (bar with "[$] [$]"). iApply (step_fupdN_wand with "[$]").
+    clear k. iIntros "(Hsup&_&_&_&HP) HE %k Hle".
+    iApply (fupd_to_bupd_except0_plain with "[$] [$]"). iMod "HP".
+    clear k. iIntros "!> %k Hle HE".
+    iApply ("HP" with "[$] [$] [$]").
   Qed.
 
 End plain_unfolding.
